Finish multi-rule programs

platform/tests/XmlTest2Driver.v
@@ -1,1 +1,128 @@
-Require Export XmlProg.
+Require Import Bedrock Xml XmlProg.
+
+Module M.
+  Definition ts := {| Name := "params";
+    Address := ((1024 * 1024 + 50) * 4)%N;
+    Schema := "key" :: "value" :: nil
+  |} :: nil.
+
+  Definition pr := (
+    Match
+      "methodCall"/(
+        "methodName"/"get"
+        & "params"/(
+          "param"/(
+            "value"/(
+              "string"/$"key"
+            )
+          )
+        )
+      )
+    Do
+      From "params" Where ("key" = $"key")
+        Write <*> "methodResponse" </>
+          <*> "params" </>
+            <*> "param" </>
+              <*> "value" </>
+                <*> "array" </>
+                  <*> "data" </>
+                    <*> "value" </>
+                      <*> "int" </>
+                        "1"
+                      </>
+                    </>,
+                    <*> "value" </>
+                      <*> "string" </>
+                        "Value is"
+                      </>
+                    </>,
+                    <*> "value" </>
+                      <*> "string" </>
+                        ^"value"
+                      </>
+                    </>
+                  </>
+                </>
+              </>
+            </>
+          </>
+        </>
+    end;;
+    Match
+      "methodCall"/(
+        "methodName"/"set"
+        & "params"/(
+          "param"/(
+            "value"/(
+              "string"/$"key"
+            )
+          );;
+          "param"/(
+            "value"/(
+              "string"/$"value"
+            )
+          )
+        )
+      )
+    Do
+      Insert "params" ($"key", $"value");;
+      Write <*> "methodResponse" </>
+        <*> "params" </>
+          <*> "param" </>
+            <*> "value" </>
+              <*> "array" </>
+                <*> "data" </>
+                  <*> "value" </>
+                    <*> "int" </>
+                      "1"
+                    </>
+                  </>,
+                  <*> "value" </>
+                    <*> "string" </>
+                      "OK"
+                    </>
+                  </>,
+                  <*> "value" </>
+                    <*> "int" </>
+                      "1"
+                    </>
+                  </>
+                </>
+              </>
+            </>
+          </>
+        </>
+      </>
+    end
+  )%program.
+
+  Theorem wellFormed : wf ts pr.
+    wf.
+  Qed.
+
+  Theorem notTooGreedy : (reserved pr <= 38)%nat.
+    compute; omega.
+  Qed.
+
+  Definition buf_size := 1024%N.
+
+  Theorem buf_size_lower : (buf_size >= 2)%N.
+    discriminate.
+  Qed.
+    
+  Theorem buf_size_upper : (buf_size * 4 < Npow2 32)%N.
+    reflexivity.
+  Qed.
+
+  Definition heapSize := (1024 * 1024)%N.
+
+  Theorem ND : NoDup (Names ts).
+    NoDup.
+  Qed.
+
+  Theorem goodSchema : twfs ts.
+    goodSchema.
+  Qed.
+End M.
+
+Module E := Make(M).
